

ESE 650, SPRING 2023

HOMEWORK 1

ANH NGUYEN [TUNA28NG@SEAS]

Solution 1 (Time spent: 10 hour). See the code on Gradescope

Solution 2 (Time spent: 8 hour). (a) See the code on Gradescope.

(b) We have

$$\begin{aligned}
 \xi_k(x, x') &= P(X_k = x, X_{k+1} = x' | Y_1, \dots, Y_t, \lambda) \\
 &= \frac{P(X_k = x, X_{k+1} = x', Y_1, \dots, Y_t, \lambda)}{P(Y_1, \dots, Y_t, \lambda)} \\
 &= \frac{P(Y_1, \dots, Y_t, \lambda | X_k = x, X_{k+1} = x') P(X_k = x, X_{k+1} = x')}{P(Y_1, \dots, Y_t, \lambda)}
 \end{aligned}$$

The numerator:

$$\begin{aligned}
 &P(Y_1, \dots, Y_t | X_k = x, X_{k+1} = x') P(X_{k+1} = x' | X_k = x) P(X_k = x) \\
 &= P(Y_1, \dots, Y_k | X_k = x, X_{k+1} = x') P(Y_{k+1}, \dots, Y_t | X_k = x, X_{k+1} = x') P(X_{k+1} = x' | X_k = x) P(X_k = x) \\
 &= P(Y_1, \dots, Y_k | X_k = x) P(Y_{k+1}, \dots, Y_t | X_{k+1} = x') P(X_{k+1} = x' | X_k = x) P(X_k = x) \text{ following Markov property} \\
 &= \frac{P(Y_1, \dots, Y_k, X_k = x)}{P(X_k = x)} P(Y_{k+1} | X_{k+1} = x') P(Y_{k+2}, \dots, Y_t | X_{k+1} = x') P(X_{k+1} = x' | X_k = x) P(X_k = x) \\
 &= P(Y_1, \dots, Y_k, X_k = x) P(Y_{k+1} | X_{k+1} = x') P(Y_{k+2}, \dots, Y_t | X_{k+1} = x') P(X_{k+1} = x' | X_k = x)
 \end{aligned}$$

Thus,

$$\xi_k(x, x') = \eta \alpha_k(x) T_{x, x'} M_{x', y_{k+1}} \beta_{k+1}(x')$$

where $\eta^{-1} = P(Y_1, \dots, Y_t, \lambda)$

(c) See the code on Gradescope

Solution 3 (Time spent: 4 hour). a) Compute probabilities:

(1)

$$\begin{aligned} P(X_{k+1} = x_j | X_k = x_i, Y_1, \dots, Y_t) &= \frac{P(X_{k+1} = x_j, X_k = x_i, Y_1, \dots, Y_t)}{P(X_k = x_i, Y_1, \dots, Y_t)} \\ &= \frac{P(Y_1, \dots, Y_t | X_k = x_i, X_{k+1} = x_j) P(X_k = x_i, X_{k+1} = x_j)}{P(X_k = x_i | Y_1, \dots, Y_t) P(Y_1, \dots, Y_t)} \end{aligned}$$

Here, the denominator can be easily compute from the derivation of the smoothing problem (section 2.4.4 in Chapter 2 note):

$$P(X_k = x_i | Y_1, \dots, Y_t) P(Y_1, \dots, Y_t) = \beta_k(x) \alpha_k(x)$$

The numerator:

$$\begin{aligned} &(P(Y_1, \dots, Y_k | X_k = x_i, X_{k+1} = x_j) P(Y_{k+1}, \dots, Y_t | X_k = x_i, X_{k+1} = x_j)) \times \\ &(P(X_{k+1} = x_j | X_k = x_i) P(X_k = x_i)) \end{aligned}$$

From Markovian property, Y_1, \dots, Y_k is not dependent on $X_{k+1} = x_j$, and all the future observations Y_{k+1}, \dots, Y_t can relate to $X_k = x_i$ through $X_{k+1} = x_j$. So we can write the first term in the numerator as follows:

$$\begin{aligned} &(P(Y_1, \dots, Y_k | X_k = x_i) P(Y_{k+1}, \dots, Y_t | X_{k+1} = x_j)) \\ &= \frac{P(Y_1, \dots, Y_k, X_k = x_i)}{P(X_k = x_i)} P(Y_{k+1} | X_{k+1} = x_j) P(Y_{k+2}, \dots, Y_t | X_{k+1} = x_j) \end{aligned}$$

Bring all the together and cancel out $P(X_k = x_i)$ we have:

$$\begin{aligned} P(X_{k+1} = x_j | X_k = x_i, Y_1, \dots, Y_t) &= \frac{\alpha_k(x) M_{ij} \beta_{k+1}(x) T_{ij}}{\beta_k(x) \alpha_k(x)} \\ &= \frac{M_{ij} \beta_{k+1}(x) T_{ij}}{\beta_k(x)} \end{aligned}$$

(2)

$$\begin{aligned} &P(X_k = x_i | X_{k+1} = x_j, Y_1, \dots, Y_t) \\ &= \frac{P(X_{k+1} = x_j, X_k = x_i, Y_1, \dots, Y_t)}{P(X_{k+1} = x_j, Y_1, \dots, Y_t)} \end{aligned}$$

The numerator here is computed similarly to last question. And the denominator:

$$P(X_{k+1} = x_j | Y_1, \dots, Y_t) P(Y_1, \dots, Y_t) = \beta_{k+1}(x) \alpha_{k+1}(x)$$

Thus,

$$\begin{aligned}
 P(X_{k+1} = x_j | X_k = x_i, Y_1, \dots, Y_t) &= \frac{\alpha_k(x) M_{ij} \beta_{k+1}(x) T_{ij}}{\beta_{k+1}(x) \alpha_{k+1}(x)} \\
 &= \frac{\alpha_k(x) M_{ij} T_{ij}}{\alpha_{k+1}(x)} \\
 (3) \quad & \\
 P(X_{k-1} = x_i, X_k = x_j, X_{k+1} = x_l | Y_1, \dots, Y_t) \\
 &= \frac{P(X_{k-1} = x_i, X_k = x_j, X_{k+1} = x_l, Y_1, \dots, Y_t)}{P(Y_1, \dots, Y_t)} \\
 &= \frac{P(Y_1, \dots, Y_t | X_{k-1} = x_i, X_k = x_j, X_{k+1} = x_l) P(X_{k-1} = x_i, X_k = x_j, X_{k+1} = x_l)}{P(Y_1, \dots, Y_t)} \\
 &= \frac{P(Y_1, \dots, Y_t | X_{k-1} = x_i, X_k = x_j, X_{k+1} = x_l) P(X_{k-1} = x_i, X_k = x_j, X_{k+1} = x_l)}{P(Y_1, \dots, Y_t)}
 \end{aligned}$$

The numerator:

$$\begin{aligned}
 &P(Y_1, \dots, Y_t | X_{k-1} = x_i, X_k = x_j, X_{k+1} = x_l) P(X_{k-1} = x_i, X_k = x_j, X_{k+1} = x_l) \\
 &= P(Y_1, \dots, Y_{k-1} | X_{k-1} = x_i) P(Y_k | X_k = x_j) P(Y_{k+1} | X_{k+1} = x_l) P(Y_{k+2}, \dots, Y_t | X_{k+1} = x_l) \times \\
 &\quad P(X_{k+1} = x_l | X_k = x_j) P(X_k = x_j | X_{k-1} = x_i) P(X_{k-1} = x_i) \\
 &= \frac{P(Y_1, \dots, Y_{k-1}, X_{k-1} = x_i)}{P(X_{k-1} = x_i)} P(Y_k | X_k = x_j) P(Y_{k+1} | X_{k+1} = x_l) P(Y_{k+2}, \dots, Y_t | X_{k+1} = x_l) \times \\
 &\quad P(X_{k+1} = x_l | X_k = x_j) P(X_k = x_j | X_{k-1} = x_i) P(X_{k-1} = x_i)
 \end{aligned}$$

Thus,

$$\begin{aligned}
 &P(X_{k-1} = x_i, X_k = x_j, X_{k+1} = x_l | Y_1, \dots, Y_t) \\
 &= \frac{\alpha_{k-1}(x) M_{jl} M_{l(l+1)} \beta_{k+1}(x) T_{jl} T_{ij}}{P(Y_1, \dots, Y_t)}
 \end{aligned}$$

where the denominator: $P(Y_1, \dots, Y_t) = \sum_x \alpha_t(x)$

Solution 4 (Time spent: 3 hour). (a)

$$\begin{aligned}\hat{X} &= a_1 Y_1 + a_2 Y_2 = (a_1 + 2a_2)X + a_1 e_1 + a_2 e_2 \\ E[\hat{X}] &= E[(a_1 + 2a_2)X + a_1 e_1 + a_2 e_2] = (a_1 + 2a_2)X\end{aligned}$$

To make sure the estimate \hat{X} is unbiased, we need $E[\hat{X}] = X$, thus

$$\begin{aligned}(a_1 + 2a_2)X &= X \\ a_1 &= 1 - 2a_2\end{aligned}$$

We have the MSE

$$\begin{aligned}E[(X - \hat{X})^2] &= E[(X - (a_1 + 2a_2)X - a_1 e_1 - a_2 e_2)^2] \\ &= E[(-(1 - 2a_2)e_1 - a_2 e_2)^2] \\ &= (1 - 2a_2)^2 \sigma_1^2 + a_2^2 \sigma_2^2 \\ &= (1 - 4a_2 + 4a_2^2) \sigma_1^2 + a_2^2 \sigma_2^2\end{aligned}$$

To minimize this MSE, we derive the above equation and find the values of a_1 and a_2 that make this first-order derivative equal 0

$$\begin{aligned}\frac{dE[(X - \hat{X})^2]}{da_2} &= (-4 + 8a_2) \sigma_1^2 + 2a_2 \sigma_2^2 = 0 \\ -4\sigma_1^2 + 2a_2(4\sigma_1^2 + \sigma_2^2) &= 0\end{aligned}$$

$$\frac{d^2 E[(X - \hat{X})^2]}{da_2^2} = 2(4\sigma_1^2 + \sigma_2^2) > 0$$

$$\begin{aligned}a_2 &= \frac{2\sigma_1^2}{4\sigma_1^2 + \sigma_2^2} \\ a_1 &= 1 - \frac{4\sigma_1^2}{4\sigma_1^2 + \sigma_2^2} = \frac{\sigma_2^2}{4\sigma_1^2 + \sigma_2^2} \\ \hat{X} &= \frac{\sigma_2^2}{4\sigma_1^2 + \sigma_2^2} Y_1 + \frac{2\sigma_1^2}{4\sigma_1^2 + \sigma_2^2} Y_2\end{aligned}$$

This estimator has variance

$$\begin{aligned}\sigma_{\hat{X}}^2 &= a_1^2 \sigma_1^2 + a_2^2 \sigma_2^2 \\ &= \frac{\sigma_2^4}{(4\sigma_1^2 + \sigma_2^2)^2} \sigma_1^2 + \frac{4\sigma_1^4}{(4\sigma_1^2 + \sigma_2^2)^2} \sigma_2^2 \\ &= \frac{\sigma_1^2 \sigma_2^2}{4\sigma_1^2 + \sigma_2^2}\end{aligned}$$

(b)

(i) If $\sigma_2 \gg \sigma_1$ then the measurement Y_2 gets less weight, and the estimator mathematically mainly depends on Y_1 . This is correct with the intuition that if this measurement is too noisy, we should rely less upon it.

(ii) If $\sigma_2 = \sigma_1$, the 2 measurements have the same variance of noise distribution, and $\hat{X} = \frac{1}{5}Y_1 + \frac{2}{5}Y_2$. This means Y_2 is weighted twice Y_1 . We would also have $\sigma_{\hat{X}^2} = \sigma_1^2/5$.

(iii) If $\sigma_1 \gg \sigma_2$, this is similar to (i), and we would rely less on the measurement Y_1 because of the much larger noise variance of this measurement.